Lecture 1 and 2

teaching/eutypes2018/code/pure-fun/AppendLength.fst
@@ -3,31 +3,31 @@ module AppendLength
 open FStar.List.Tot.Base
 
 // BEGIN: append
-let rec append (#a:Type) (xs ys : list a) : Tot (list a) 
-  = match xs with
-    | []       -> ys
-    | x :: xs' -> x :: append xs' ys
+let rec append (#a:Type) (xs ys : list a) : Tot (list a) = 
+  match xs with
+  | []       -> ys
+  | x :: xs' -> x :: append xs' ys
 // END: append
 
 // BEGIN: append_length
 let rec append_length (#a:Type) (xs ys : list a) 
   : Pure unit
       (requires True)
-      (ensures  (fun _ -> length (append xs ys) = length xs + length ys))
+      (ensures  (fun _ -> length (append xs ys) = length xs + length ys)) =
       
-  = match xs with
-    | []       -> ()
-    | x :: xs' -> append_length xs' ys
+  match xs with
+  | []       -> ()
+  | x :: xs' -> append_length xs' ys
 // END: append_length
 
 // BEGIN: append_length_lemma
 let rec append_length_lemma (#a:Type) (xs ys : list a) 
 
-    : Lemma (length (append xs ys) = length xs + length ys)
+    : Lemma (length (append xs ys) = length xs + length ys) =
     
-    = match xs with
-      | []       -> ()
-      | x :: xs' -> append_length_lemma xs' ys
+    match xs with
+    | []       -> ()
+    | x :: xs' -> append_length_lemma xs' ys
 // END: append_length_lemma
 
 (*
